PossiblyInfiniteTrees/PossiblyInfiniteList/PossiblyInfiniteList.lean
@@ -1,69 +1,206 @@
+-- We mimic Mathlib's Stream'.Seq a lot here.
+-- Still I keep this separate to see better what is actually needed
+-- and since what we need should be simple enough.
+
 import PossiblyInfiniteTrees.PossiblyInfiniteList.InfiniteList
+
+def InfiniteList.no_holes (l : InfiniteList (Option α)) : Prop := ∀ n : Nat, l.get n = none -> l.get n.succ = none
 
 structure PossiblyInfiniteList (α : Type u) where
   infinite_list : InfiniteList (Option α)
-  no_holes : ∀ n : Nat, infinite_list n ≠ none -> ∀ m : Fin n, infinite_list m ≠ none
+  no_holes : infinite_list.no_holes
 
 namespace PossiblyInfiniteList
-  def empty : PossiblyInfiniteList α := {
-    infinite_list := fun _ => none
-    no_holes := by intros; contradiction
-  }
 
-  def fromList : List α -> PossiblyInfiniteList α
-  | .nil => {
+  def empty : PossiblyInfiniteList α where
     infinite_list := fun _ => none
-    no_holes := by simp
-  }
-  | .cons a as => {
-    infinite_list := fun n => match n with
-    | .zero => a
-    | .succ n => (fromList as).infinite_list n
-    no_holes := by
-      have no_holes_rec := (fromList as).no_holes
-      intro n
-      cases n with
-      | zero => simp
-      | succ n =>
-        simp
-        intro h m
-        cases eq : m.val with
-        | zero => simp
-        | succ m' =>
-          simp
-          specialize no_holes_rec n h ⟨m-1, by
-            have isLt := m.isLt
-            rw [eq] at isLt
-            simp at isLt
-            have : m - 1 = m' := by rw [eq]; simp
-            rw [this]
-            exact isLt
-          ⟩
-          simp only [eq] at no_holes_rec
-          simp at no_holes_rec
-          exact no_holes_rec
-  }
+    no_holes := by intro _ _; rfl
 
-  theorem eq_iff_same_on_all_indices (as bs : PossiblyInfiniteList α) : as = bs ↔ ∀ n, as.infinite_list n = bs.infinite_list n := by
+  def get? (l : PossiblyInfiniteList α) (n : Nat) : Option α := l.infinite_list.get n
+
+  theorem get?_empty {α} : ∀ {n}, (@PossiblyInfiniteList.empty α).get? n = none := by intro _; rfl
+
+  theorem no_holes' {l : PossiblyInfiniteList α} : ∀ n, l.get? n = none -> l.get? n.succ = none := by exact l.no_holes
+
+  instance : Membership α (PossiblyInfiniteList α) where
+    mem l a := some a ∈ l.infinite_list
+
+  theorem mem_iff {l : PossiblyInfiniteList α} : ∀ {e}, e ∈ l ↔ ∃ n, l.get? n = some e := by rfl
+
+  theorem get?_eq_none_of_le_of_eq_none {l : PossiblyInfiniteList α} {n : Nat} :
+      l.get? n = none -> ∀ m, n ≤ m -> l.get? m = none := by
+    intro h
+    have : ∀ k, l.get? (n + k) = none := by
+      intro k
+      induction k with
+      | zero => exact h
+      | succ k ih => apply l.no_holes; exact ih
+    intro m le
+    rcases Nat.exists_eq_add_of_le le with ⟨k, k_eq⟩
+    rw [k_eq]
+    exact this k
+
+  def drop (l : PossiblyInfiniteList α) (n : Nat) : PossiblyInfiniteList α where
+    infinite_list := l.infinite_list.drop n
+    no_holes := by intro n'; rw [InfiniteList.get_drop, InfiniteList.get_drop, Nat.add_succ]; exact l.no_holes (n + n')
+
+  theorem get?_drop {l : PossiblyInfiniteList α} {n i : Nat} : (l.drop n).get? i = l.get? (n + i) := by rfl
+
+  theorem ext {l1 l2 : PossiblyInfiniteList α} : (∀ n, l1.get? n = l2.get? n) -> l1 = l2 := by
+    intro h; rw [PossiblyInfiniteList.mk.injEq]; apply InfiniteList.ext; exact h
+
+  theorem ext_iff {l1 l2 : PossiblyInfiniteList α} : l1 = l2 ↔ (∀ n, l1.get? n = l2.get? n) := by
     constructor
-    . intro h _
-      rw [h]
-    . intro h
-      rw [PossiblyInfiniteList.mk.injEq]
-      apply funext
-      exact h
+    . intro h _; rw [h]
+    . exact ext
 
-  theorem get_fromList_eq_list_getElem (l : List α) : ∀ n, (fromList l).infinite_list n = l[n]? := by
-    induction l with
-    | nil => simp [fromList]
-    | cons a as ih =>
+  theorem drop_zero {l : PossiblyInfiniteList α} : l.drop 0 = l := by
+    rw [PossiblyInfiniteList.mk.injEq]; exact InfiniteList.drop_zero
+
+  def cons (hd : α) (tl : PossiblyInfiniteList α) : PossiblyInfiniteList α where
+    infinite_list := InfiniteList.cons (.some hd) tl.infinite_list
+    no_holes := by
       intro n
-      unfold fromList
       cases n with
-      | zero => simp
+      | zero => intro contra; rw [← InfiniteList.head.eq_def, InfiniteList.head_cons] at contra; simp at contra
       | succ n =>
-        simp
-        apply ih
+        rw [← InfiniteList.tail.eq_def, InfiniteList.tail_cons]
+        rw [← InfiniteList.tail.eq_def, InfiniteList.tail_cons]
+        exact tl.no_holes n
+
+  theorem get?_cons_zero {hd : α} {tl : PossiblyInfiniteList α} : (cons hd tl).get? 0 = .some hd := by unfold get?; unfold cons; rw [InfiniteList.get_cons_zero]
+  theorem get?_cons_succ {hd : α} {tl : PossiblyInfiniteList α} : ∀ n, (cons hd tl).get? n.succ = tl.get? n := by intro n; unfold get?; unfold cons; rw [InfiniteList.get_cons_succ]
+
+  def head (l : PossiblyInfiniteList α) : Option α := l.infinite_list.head
+  def tail (l : PossiblyInfiniteList α) : PossiblyInfiniteList α where
+    infinite_list := l.infinite_list.tail
+    no_holes := by intro n; rw [InfiniteList.get_tail, InfiniteList.get_tail]; exact l.no_holes n.succ
+
+  theorem head_eq {l : PossiblyInfiniteList α} : l.head = l.get? 0 := by rfl
+
+  theorem head_cons (hd : α) (tl : PossiblyInfiniteList α) : (cons hd tl).head = hd := InfiniteList.head_cons
+  theorem tail_cons (hd : α) (tl : PossiblyInfiniteList α) : (cons hd tl).tail = tl := by simp [cons, tail, InfiniteList.tail_cons]
+
+  theorem cons_head_tail (l : PossiblyInfiniteList α) (hd : α) (h : l.head = .some hd) : l = cons hd l.tail := by rw [PossiblyInfiniteList.mk.injEq]; simp only [cons]; rw [← h]; apply InfiniteList.cons_head_tail
+
+  theorem get?_tail {l : PossiblyInfiniteList α} : ∀ n, l.tail.get? n = l.get? n.succ := by intros; rfl
+
+  theorem head_drop {l : PossiblyInfiniteList α} : ∀ {n}, (l.drop n).head = l.get? n := by intros; rfl
+  theorem tail_drop {l : PossiblyInfiniteList α} : ∀ {n}, (l.drop n).tail = l.drop n.succ := by
+    intros; unfold tail drop; apply ext; intro n; simp only [get?, InfiniteList.tail_drop]
+
+  theorem empty_iff_head_none {l : PossiblyInfiniteList α} : l = PossiblyInfiniteList.empty ↔ l.head = none := by
+    constructor
+    . intro h; rw [h]; simp [head, empty, InfiniteList.head, InfiniteList.get]
+    intro h
+    apply ext
+    intro n
+    induction n with
+    | zero => rw [get?_empty]; exact h
+    | succ n ih =>
+      rw [get?_empty] at ih
+      rw [get?_empty]
+      apply l.no_holes
+      exact ih
+
+  def map (l : PossiblyInfiniteList α) (f : α -> β) : PossiblyInfiniteList β where
+    infinite_list := l.infinite_list.map (fun o => o.map f)
+    no_holes := by intro n; simp only [InfiniteList.get_map, Option.map_eq_none_iff]; apply l.no_holes
+
+  theorem get?_map {l : PossiblyInfiniteList α} {f : α -> β} {n : Nat} : (l.map f).get? n = (l.get? n).map f := by rfl
+
+  def finite (l : PossiblyInfiniteList α) : Prop := ∃ k, l.get? k = none
+
+  theorem finite_empty {α} : (@PossiblyInfiniteList.empty α).finite := by exists 0
+
+  theorem map_finite_of_finite {l : PossiblyInfiniteList α} {f : α -> β} : l.finite -> (l.map f).finite := by
+    rintro ⟨i, h⟩; exists i; rw [get?_map, Option.map_eq_none_iff]; exact h
+
+  def toList_of_finite (l : PossiblyInfiniteList α) (fin : l.finite) : List α :=
+    let rec loop (n : Nat) : List α :=
+      match eq : l.get? n with
+      | .none => []
+      | .some a =>
+        have termination_hint : Classical.choose fin - (n + 1) < Classical.choose fin - n := by
+          apply Nat.sub_add_lt_sub _ (by simp)
+          have spec := Classical.choose_spec fin
+          apply Classical.byContradiction
+          intro contra
+          simp only [Nat.not_le] at contra
+          have contra := Nat.le_of_lt_succ contra
+          have := l.get?_eq_none_of_le_of_eq_none spec _ contra
+          rw [eq] at this
+          simp at this
+        a :: loop (n+1)
+    termination_by (Classical.choose fin) - n
+    loop 0
+
+  theorem getElem?_toList_of_finite {l : PossiblyInfiniteList α} {fin : l.finite} : ∀ {n}, (l.toList_of_finite fin)[n]? = l.get? n := by
+    have : ∀ n m, (toList_of_finite.loop l fin m)[n]? = l.get? (m + n) := by
+      intro n
+      induction n with
+      | zero =>
+        intro m; unfold toList_of_finite.loop
+        split
+        case h_1 eq => simp [eq]
+        case h_2 eq => simp [eq]
+      | succ n ih =>
+        intro m; unfold toList_of_finite.loop; specialize ih (m+1); rw [Nat.add_comm n 1, ← Nat.add_assoc, ← ih]
+        split
+        case h_2 eq => rw [Nat.add_comm 1 n, List.getElem?_cons_succ]
+        case h_1 eq =>
+          unfold toList_of_finite.loop
+          split
+          . simp
+          case h_2 eq2 =>
+            have := l.no_holes m eq
+            unfold PossiblyInfiniteList.get? at eq2
+            rw [this] at eq2
+            simp at eq2
+    intro n
+    unfold toList_of_finite
+    rw [this n 0, Nat.zero_add]
+
+  theorem mem_toList_of_finite {l : PossiblyInfiniteList α} {fin : l.finite} : ∀ {e}, e ∈ l.toList_of_finite fin ↔ e ∈ l := by
+    intro e
+    rw [List.mem_iff_getElem?]
+    constructor
+    . intro h; rcases h with ⟨i, h⟩; exists i; rw [getElem?_toList_of_finite] at h; exact h
+    . intro h; rcases h with ⟨i, h⟩; exists i; rw [getElem?_toList_of_finite]; exact h
+
+  theorem map_toList_of_finite {l : PossiblyInfiniteList α} {fin : l.finite} {f : α -> β} : (l.toList_of_finite fin).map f = (l.map f).toList_of_finite (map_finite_of_finite fin) := by
+    apply List.ext_getElem?
+    intro i
+    rw [List.getElem?_map, getElem?_toList_of_finite, getElem?_toList_of_finite]
+    rfl
+
+  theorem toList_of_finite_empty_iff {l : PossiblyInfiniteList α} {fin : l.finite} : l.toList_of_finite fin = [] ↔ l = PossiblyInfiniteList.empty := by
+    constructor
+    . intro eq
+      apply PossiblyInfiniteList.ext
+      rw [List.ext_getElem?_iff] at eq
+      intro n
+      specialize eq n
+      rw [getElem?_toList_of_finite] at eq
+      rw [eq]
+      rfl
+    . intro eq
+      apply List.ext_getElem?
+      intro n
+      rw [getElem?_toList_of_finite]
+      rw [eq]
+      rw [get?_empty, List.getElem?_nil]
+
+  def from_list (l : List α) : PossiblyInfiniteList α where
+    infinite_list := fun n => l[n]?
+    no_holes := by intro n; simp only [InfiniteList.get]; simp only [List.getElem?_eq_none_iff]; exact Nat.le_succ_of_le
+
+  theorem get?_from_list {l : List α} : ∀ {n}, (from_list l).get? n = l[n]? := by intros; rfl
+
+  theorem finite_from_list {l : List α} : (from_list l).finite := by exists l.length; rw [get?_from_list]; apply List.getElem?_eq_none; simp
+
+  theorem toList_of_finite_after_from_list {l : List α} : (from_list l).toList_of_finite finite_from_list = l := by
+    apply List.ext_getElem?; intro i; rw [getElem?_toList_of_finite, get?_from_list]
 
 end PossiblyInfiniteList
 
