PossiblyInfiniteTrees/PossiblyInfiniteTree/InfiniteTree.lean
@@ -2,64 +2,85 @@ import BasicLeanDatastructures.Set.Basic
 
 import PossiblyInfiniteTrees.PossiblyInfiniteList.PossiblyInfiniteList
 
--- NOTE: all finite lists indicating positions are right to left; infinite lists left to right (don't ask)
-
 def InfiniteTreeSkeleton (α : Type u) := (List Nat) -> α
 
 namespace InfiniteTreeSkeleton
 
-  def children (tree : InfiniteTreeSkeleton α) (node : List Nat) : InfiniteList α := fun n => tree (n :: node)
+  def get (t : InfiniteTreeSkeleton α) (ns : List Nat) : α := t ns
 
-  def branch_addresses_through (node : List Nat) : Set (InfiniteList Nat) := fun nodes =>
-    (nodes.take node.length).reverse = node
+  def drop (t : InfiniteTreeSkeleton α) (ns : List Nat) : InfiniteTreeSkeleton α := fun ns' => t.get (ns ++ ns')
 
-  def branch_for_address (tree : InfiniteTreeSkeleton α) (nodes : InfiniteList Nat) : InfiniteList α := fun n => tree (nodes.take n).reverse
+  theorem drop_eq {t : InfiniteTreeSkeleton α} {ns : List Nat} : t.drop ns = fun ns' => t.get (ns ++ ns') := rfl
 
-  def branches_through (tree : InfiniteTreeSkeleton α) (node : List Nat) : Set (InfiniteList α) :=
-    (branch_addresses_through node).map tree.branch_for_address
+  theorem drop_nil {t : InfiniteTreeSkeleton α} : t.drop [] = t := by rfl
 
-  def branches (tree : InfiniteTreeSkeleton α) : Set (InfiniteList α) := tree.branches_through []
+  theorem get_drop {t : InfiniteTreeSkeleton α} {ns ns' : List Nat} : (t.drop ns).get ns' = t.get (ns ++ ns') := by rfl
 
-  theorem branch_addresses_through_eq_union_branch_addresses_through_successors (node : List Nat) : branch_addresses_through node = fun nodes => ∃ (i : Nat), nodes ∈ branch_addresses_through (i :: node) := by
-    unfold branch_addresses_through
-    apply Set.ext
-    simp only [List.length_cons, List.reverse_eq_cons_iff, Membership.mem]
-    intro nodes
+  theorem drop_drop {t : InfiniteTreeSkeleton α} {ns ns' : List Nat} : (t.drop ns).drop ns' = t.drop (ns ++ ns') := by
+    rw [drop_eq]; simp only [get_drop]; rw [drop_eq]; simp
+
+  theorem ext {t1 t2 : InfiniteTreeSkeleton α} : (∀ ns, t1.get ns = t2.get ns) -> t1 = t2 := by
+    apply funext
+
+  theorem ext_iff {t1 t2 : InfiniteTreeSkeleton α} : t1 = t2 ↔ (∀ ns, t1.get ns = t2.get ns) := by
     constructor
-    . intro h
-      exists nodes node.length
-      unfold InfiniteList.take
-      rw [List.append_cancel_right_eq]
-      rw [← List.reverse_eq_iff]
-      exact h
-    . intro h
-      rcases h with ⟨i, h⟩
-      unfold InfiniteList.take at h
-      rw [← List.reverse_inj] at h
-      rw [List.reverse_append] at h
-      rw [List.reverse_append] at h
-      simp only [List.reverse_cons, List.reverse_nil, List.nil_append, List.cons_append, List.reverse_reverse] at h
-      rw [List.cons.injEq] at h
-      exact h.right
+    . intro h _; rw [h]
+    . exact ext
 
-  theorem branches_through_eq_union_branches_through_successors (tree : InfiniteTreeSkeleton α) (node : List Nat) : tree.branches_through node = fun b => ∃ (i : Nat), b ∈ tree.branches_through (i :: node) := by
-    unfold branches_through
-    rw [branch_addresses_through_eq_union_branch_addresses_through_successors]
-    unfold Set.map
+  def node (root : α) (childTrees : InfiniteList (InfiniteTreeSkeleton α)) : InfiniteTreeSkeleton α
+  | .nil => root
+  | .cons hd tl => childTrees hd tl
+
+  theorem get_node_nil {root : α} {childTrees : InfiniteList (InfiniteTreeSkeleton α)} : (node root childTrees).get [] = root := by rfl
+  theorem get_node_cons {root : α} {childTrees : InfiniteList (InfiniteTreeSkeleton α)} : ∀ n ns, (node root childTrees).get (n :: ns) = (childTrees.get n).get ns := by intro n ns; rfl
+
+  def root (t : InfiniteTreeSkeleton α) : α := t.get []
+  def childTrees (t : InfiniteTreeSkeleton α) : InfiniteList (InfiniteTreeSkeleton α) := fun n ns => t.get (n::ns)
+
+  theorem root_drop {t : InfiniteTreeSkeleton α} {ns : List Nat} : (t.drop ns).root = t.get ns := by
+    unfold root; rw [get_drop]; simp
+
+  theorem root_node {root : α} {childTrees : InfiniteList (InfiniteTreeSkeleton α)} : (node root childTrees).root = root := by rfl
+  theorem childTrees_node {root : α} {childTrees : InfiniteList (InfiniteTreeSkeleton α)} : (node root childTrees).childTrees = childTrees := by rfl
+
+  theorem node_root_childTrees (t : InfiniteTreeSkeleton α) : t = node t.root t.childTrees := by apply ext; intro ns; cases ns; rw [get_node_nil]; rfl; rw [get_node_cons]; rfl
+
+  theorem get_childTrees {t : InfiniteTreeSkeleton α} : ∀ n, (t.childTrees.get n) = t.drop [n] := by intros; rfl
+  theorem get_get_childTrees {t : InfiniteTreeSkeleton α} : ∀ n ns, (t.childTrees.get n).get ns = t.get (n::ns) := by intros; rfl
+
+  theorem drop_node_cons {root : α} {childTrees : InfiniteList (InfiniteTreeSkeleton α)} {n : Nat} {ns : List Nat} :
+      (node root childTrees).drop (n::ns) = (childTrees.get n).drop ns := by
+    rfl
+
+  def childNodes (t : InfiniteTreeSkeleton α) : InfiniteList α := t.childTrees.map root
+
+  theorem get_childNodes {t : InfiniteTreeSkeleton α} {n : Nat} : t.childNodes.get n = t.get [n] := by rfl
+
+  def branchForAddress (t : InfiniteTreeSkeleton α) (ns : InfiniteList Nat) : InfiniteList α := fun n => t.get (ns.take n)
+  def branches (t : InfiniteTreeSkeleton α) : Set (InfiniteList α) := fun b => ∃ ns, b = t.branchForAddress ns
+
+  theorem get_branchForAddress {t : InfiniteTreeSkeleton α} {ns : InfiniteList Nat} {n : Nat} : (t.branchForAddress ns).get n = t.get (ns.take n) := by rfl
+  theorem head_branchForAddress {t : InfiniteTreeSkeleton α} {ns : InfiniteList Nat} : (t.branchForAddress ns).head = t.root := by rfl
+  theorem tail_branchForAddress {t : InfiniteTreeSkeleton α} {ns : InfiniteList Nat} : (t.branchForAddress ns).tail = (t.childTrees.get ns.head).branchForAddress ns.tail := by rfl
+  theorem branchForAddress_cons {t : InfiniteTreeSkeleton α} {n : Nat} {ns : InfiniteList Nat} : t.branchForAddress (InfiniteList.cons n ns) = InfiniteList.cons t.root ((t.childTrees.get n).branchForAddress ns) := by
+    conv => left; rw [InfiniteList.cons_head_tail (t.branchForAddress (InfiniteList.cons n ns))]
+    rw [head_branchForAddress, tail_branchForAddress, InfiniteList.head_cons, InfiniteList.tail_cons]
+
+  theorem branches_node {root : α} {childTrees : InfiniteList (InfiniteTreeSkeleton α)} :
+      (node root childTrees).branches = fun b => b.head = root ∧ ∃ n, b.tail ∈ (childTrees.get n).branches := by
     apply Set.ext
     intro b
     constructor
-    . intro ⟨nodes, h, b_eq⟩
-      rcases h with ⟨i, h⟩
-      exists i
-      exists nodes
-    . intro h
-      rcases h with ⟨i, nodes, h⟩
-      exists nodes
+    . rintro ⟨ns, h⟩
       constructor
-      . exists i
-        exact h.left
-      . exact h.right
+      . rw [h, head_branchForAddress, root_node]
+      . exists ns.head, ns.tail
+        rw [h, tail_branchForAddress, childTrees_node]
+    . rintro ⟨head_eq, n, ns, tail_eq⟩
+      exists InfiniteList.cons n ns
+      rw [branchForAddress_cons, root_node, childTrees_node]
+      rw [InfiniteList.cons_head_tail b]
+      rw [head_eq, tail_eq]
 
 end InfiniteTreeSkeleton
 
