PossiblyInfiniteTrees/PossiblyInfiniteTree/PossiblyInfiniteTree.lean
@@ -1,170 +1,410 @@
 import PossiblyInfiniteTrees.PossiblyInfiniteTree.InfiniteTree
 
+def InfiniteTreeSkeleton.no_orphans (t : InfiniteTreeSkeleton (Option α)) : Prop :=
+  ∀ ns : List Nat, t.get ns = none -> ∀ n, (t.drop ns).childNodes.get n = none
+
+theorem InfiniteTreeSkeleton.no_orphans_closure {t : InfiniteTreeSkeleton (Option α)} (no_orph : t.no_orphans) :
+    ∀ ns : List Nat, t.get ns = none -> ∀ ns', (t.drop ns).get ns' = none := by
+  intro ns eq_none ns'
+  induction ns' generalizing ns with
+  | nil => rw [get_drop, List.append_nil]; exact eq_none
+  | cons hd tl ih =>
+    specialize ih (ns ++ [hd]) (by
+      have := no_orph ns eq_none hd
+      rw [get_childNodes, get_drop] at this
+      exact this)
+    rw [get_drop, List.append_assoc, List.singleton_append] at ih
+    rw [get_drop]
+    exact ih
+
 structure PossiblyInfiniteTree (α : Type u) where
   infinite_tree : InfiniteTreeSkeleton (Option α)
   no_orphans :
-    ∀ node : List Nat, infinite_tree node ≠ none ->
-    ∀ parent : { l : List Nat // ∃ diff, diff ++ l = node }, infinite_tree parent ≠ none
+    ∀ ns : List Nat, infinite_tree.get ns = none -> ∀ n, (infinite_tree.drop ns).childNodes.get n = none
   no_holes_in_children :
-    ∀ node : List Nat, ∀ n : Nat, (infinite_tree.children node) n ≠ none ->
-    ∀ m : Fin n, (infinite_tree.children node) m ≠ none
+    ∀ ns : List Nat, (infinite_tree.drop ns).childNodes.no_holes
 
 namespace PossiblyInfiniteTree
 
-  def get (tree : PossiblyInfiniteTree α) (node : List Nat) : Option α := tree.infinite_tree node
+  def empty : PossiblyInfiniteTree α where
+    infinite_tree := fun _ => none
+    no_orphans := by intro _ _ _; rw [InfiniteTreeSkeleton.get_childNodes, InfiniteTreeSkeleton.get_drop]; simp [InfiniteTreeSkeleton.get]
+    no_holes_in_children := by intro _ _ _; rw [InfiniteTreeSkeleton.get_childNodes, InfiniteTreeSkeleton.get_drop]; simp [InfiniteTreeSkeleton.get]
 
-  def children (tree : PossiblyInfiniteTree α) (node : List Nat) : PossiblyInfiniteList α := {
-    infinite_list := tree.infinite_tree.children node,
-    no_holes := by apply tree.no_holes_in_children
-  }
+  def get? (t : PossiblyInfiniteTree α) (ns : List Nat) : Option α := t.infinite_tree.get ns
 
-  theorem children_empty_of_get_eq_none (tree : PossiblyInfiniteTree α) (node : List Nat) : tree.get node = none -> tree.children node = PossiblyInfiniteList.empty := by
-    intro h
-    unfold children
-    unfold PossiblyInfiniteList.empty
-    simp
-    apply funext
-    intro index
-    have dec : Decidable (tree.infinite_tree.children node index = none) := Option.decidableEqNone
-    apply dec.byContradiction
-    intro contra
-    let parent : { l : List Nat // ∃ diff, diff ++ l = index :: node } := ⟨node, by exists [index]⟩
-    have : tree.infinite_tree parent ≠ none := by
-      apply no_orphans
-      unfold InfiniteTreeSkeleton.children at contra
-      exact contra
-    contradiction
+  theorem get?_empty {α} : ∀ {n}, (@PossiblyInfiniteTree.empty α).get? n = none := by intro _; rfl
 
-  theorem each_successor_none_of_children_empty (tree : PossiblyInfiniteTree α) (node : List Nat) : tree.children node = PossiblyInfiniteList.empty -> ∀ i, tree.get (i :: node) = none := by
-    intro h i
-    unfold get
-    unfold children at h
-    unfold PossiblyInfiniteList.empty at h
-    simp at h
-    unfold InfiniteTreeSkeleton.children at h
-    apply congr h
-    rfl
+  def drop (t : PossiblyInfiniteTree α) (ns : List Nat) : PossiblyInfiniteTree α where
+    infinite_tree := t.infinite_tree.drop ns
+    no_orphans := by intro ns'; rw [InfiniteTreeSkeleton.get_drop]; intro eq_none n; rw [InfiniteTreeSkeleton.drop_drop]; apply t.no_orphans; exact eq_none
+    no_holes_in_children := by intro ns; rw [InfiniteTreeSkeleton.drop_drop]; apply t.no_holes_in_children
 
-  theorem children_empty_of_first_successor_none (tree : PossiblyInfiniteTree α) (node : List Nat) : tree.get (0::node) = none -> tree.children node = PossiblyInfiniteList.empty := by
-    intro h
-    unfold PossiblyInfiniteList.empty
-    unfold children
-    unfold InfiniteTreeSkeleton.children
-    simp
-    apply funext
-    intro n
-    cases n with
-    | zero => exact h
-    | succ n =>
-      apply Option.decidableEqNone.byContradiction
-      intro contra
-      have no_holes := tree.no_holes_in_children node (n+1)
-      unfold children at no_holes
-      unfold InfiniteTreeSkeleton.children at no_holes
-      specialize no_holes contra ⟨0, by simp⟩
-      contradiction
+  theorem drop_nil {t : PossiblyInfiniteTree α} : t.drop [] = t := by rfl
 
-  theorem getElem_children_eq_get (tree : PossiblyInfiniteTree α) (node : List Nat) (index : Nat) : (tree.children node).infinite_list index = tree.get (index :: node) := by
-    unfold children
-    unfold get
-    unfold InfiniteTreeSkeleton.children
-    simp
+  theorem get?_drop {t : PossiblyInfiniteTree α} {ns ns' : List Nat} : (t.drop ns).get? ns' = t.get? (ns ++ ns') := by rfl
 
-  def branch_address_is_maximal (tree : PossiblyInfiniteTree α) (nodes : InfiniteList Nat) : Prop :=
-    ∀ n, tree.get (nodes.take (n+1)).reverse = none -> tree.get (0 :: (nodes.take n).reverse) = none
+  theorem drop_drop {t : PossiblyInfiniteTree α} {ns ns' : List Nat} : (t.drop ns).drop ns' = t.drop (ns ++ ns') := by simp [drop, InfiniteTreeSkeleton.drop_drop]
 
-  def branch_addresses_through (tree : PossiblyInfiniteTree α) (node : List Nat) : Set (InfiniteList Nat) := fun nodes =>
-    nodes ∈ InfiniteTreeSkeleton.branch_addresses_through node ∧ tree.branch_address_is_maximal nodes
+  theorem ext {t1 t2 : PossiblyInfiniteTree α} : (∀ ns, t1.get? ns = t2.get? ns) -> t1 = t2 := by
+    intro h; rw [PossiblyInfiniteTree.mk.injEq]; apply InfiniteTreeSkeleton.ext; exact h
 
-  def branch_for_address (tree : PossiblyInfiniteTree α) (nodes : InfiniteList Nat) : PossiblyInfiniteList α := {
-    infinite_list := tree.infinite_tree.branch_for_address nodes
-    no_holes := by
-      intro n h m
-      exact tree.no_orphans
-        (nodes.take n).reverse
-        h
-        ⟨(nodes.take m.val).reverse, by exists ((nodes.skip m.val).take (n - m.val)).reverse; rw [← List.reverse_append, InfiniteList.combine_skip_take]⟩
-  }
-
-  def branches_through (tree : PossiblyInfiniteTree α) (node : List Nat) : Set (PossiblyInfiniteList α) :=
-    (tree.branch_addresses_through node).map tree.branch_for_address
-
-  def branches (tree : PossiblyInfiniteTree α) : Set (PossiblyInfiniteList α) := tree.branches_through []
-
-  theorem branch_addresses_through_eq_union_branch_addresses_through_successors (tree : PossiblyInfiniteTree α) (node : List Nat) : tree.branch_addresses_through node = fun nodes => ∃ (i : Nat), nodes ∈ tree.branch_addresses_through (i :: node) := by
-    unfold branch_addresses_through
-    apply Set.ext
-    intro pil
-    rw [InfiniteTreeSkeleton.branch_addresses_through_eq_union_branch_addresses_through_successors]
+  theorem ext_iff {t1 t2 : PossiblyInfiniteTree α} : t1 = t2 ↔ (∀ ns, t1.get? ns = t2.get? ns) := by
     constructor
-    . intro ⟨hl, hr⟩
-      rcases hl with ⟨i, hl⟩
-      exists i
-    . intro h
-      rcases h with ⟨i, hl, hr⟩
-      constructor
-      . exists i
-      . exact hr
+    . intro h _; rw [h]
+    . exact ext
 
-  theorem branches_through_eq_union_branches_through_successors (tree : PossiblyInfiniteTree α) (node : List Nat) : tree.branches_through node = fun b => ∃ (i : Nat), b ∈ tree.branches_through (i :: node) := by
-    unfold branches_through
-    rw [branch_addresses_through_eq_union_branch_addresses_through_successors]
-    apply Set.ext
-    intro pil
+  theorem drop_empty {α} : ∀ {ns}, (@PossiblyInfiniteTree.empty α).drop ns = PossiblyInfiniteTree.empty := by
+    intro _; apply ext; intro _; rw [get?_drop, get?_empty, get?_empty]
+
+  def root (t : PossiblyInfiniteTree α) : Option α := t.infinite_tree.root
+
+  theorem root_eq {t : PossiblyInfiniteTree α} : t.root = t.get? [] := by rfl
+
+  theorem root_drop {t : PossiblyInfiniteTree α} {ns : List Nat} : (t.drop ns).root = t.get? ns := by
+    unfold root drop; simp [InfiniteTreeSkeleton.root_drop]; rfl
+
+  theorem root_empty {α} : (@PossiblyInfiniteTree.empty α).root = none := by rfl
+
+  theorem empty_iff_root_none {t : PossiblyInfiniteTree α} : t = PossiblyInfiniteTree.empty ↔ t.root = none := by
     constructor
-    . intro ⟨nodes, h, b_eq⟩
-      rcases h with ⟨i, h⟩
-      exists i
-      exists nodes
-    . intro h
-      rcases h with ⟨i, nodes, h⟩
-      exists nodes
-      constructor
-      . exists i
-        exact h.left
-      . exact h.right
+    . intro h; rw [h]; exact root_empty
+    intro h
+    rw [root_eq] at h
+    apply PossiblyInfiniteTree.ext
+    intro ns
+    induction ns generalizing t with
+    | nil => rw [h]; rfl
+    | cons n ns ih =>
+      rw [← List.singleton_append, ← get?_drop];
+      rw [ih]
+      . rfl
+      . rw [get?_drop]
+        have := t.no_orphans [] h n
+        rw [InfiniteTreeSkeleton.get_childNodes, InfiniteTreeSkeleton.get_drop] at this
+        exact this
 
-  def leaves (tree : PossiblyInfiniteTree α) : Set α := fun a => ∃ node : List Nat, tree.get node = some a ∧ tree.children node = PossiblyInfiniteList.empty
+  abbrev PossiblyInfiniteTreeWithRoot (α : Type u) := {t : PossiblyInfiniteTree α // t.root ≠ none}
 
-  def from_branch (branch : PossiblyInfiniteList α) : PossiblyInfiniteTree α := {
-    infinite_tree := fun node => if node.all (fun e => e = 0) then branch.infinite_list node.length else none
+  namespace PossiblyInfiniteTreeWithRoot
+
+    def opt_to_tree (opt : Option (PossiblyInfiniteTreeWithRoot α)) : PossiblyInfiniteTree α :=
+      match opt with
+      | .none => PossiblyInfiniteTree.empty
+      | .some t => t.val
+
+    theorem opt_to_tree_none_iff {opt : Option (PossiblyInfiniteTreeWithRoot α)} : opt = none ↔ (opt_to_tree opt).root = none := by
+      unfold opt_to_tree
+      cases opt with
+      | none => simp [root_empty]
+      | some t => simp [t.property]
+
+    def tree_to_opt (t : PossiblyInfiniteTree α) : Option (PossiblyInfiniteTreeWithRoot α) :=
+      match eq : t.root with
+      | .none => none
+      | .some r => some ⟨t, by simp [eq]⟩
+
+    theorem tree_to_opt_none_iff {t : PossiblyInfiniteTree α} : tree_to_opt t = none ↔ t.root = none := by
+      unfold tree_to_opt
+      split; simpa; simp [*]
+
+    theorem tree_to_opt_some_iff {t : PossiblyInfiniteTree α} : ∀ {t'}, tree_to_opt t = some t' ↔ t = t' ∧ t.root.isSome := by
+      unfold tree_to_opt
+      split
+      case h_1 eq => simp [eq]
+      case h_2 eq => simp [eq]
+
+    theorem tree_to_opt_after_opt_to_tree {opt : Option (PossiblyInfiniteTreeWithRoot α)} :
+        tree_to_opt (opt_to_tree opt) = opt := by
+      cases eq : opt with
+      | none => rw [tree_to_opt_none_iff, ← opt_to_tree_none_iff]
+      | some t =>
+        simp only [opt_to_tree, tree_to_opt]
+        split
+        . have := t.property; contradiction
+        . rfl
+
+    theorem opt_to_tree_after_tree_to_opt {t : PossiblyInfiniteTree α} :
+        opt_to_tree (tree_to_opt t) = t := by
+      unfold tree_to_opt
+      split
+      . simp only [opt_to_tree]; apply Eq.symm; rw [empty_iff_root_none]; assumption
+      . simp only [opt_to_tree]
+
+  end PossiblyInfiniteTreeWithRoot
+
+  def childTrees (t : PossiblyInfiniteTree α) : PossiblyInfiniteList (PossiblyInfiniteTreeWithRoot α) where
+    infinite_list := fun n => PossiblyInfiniteTreeWithRoot.tree_to_opt {
+      infinite_tree := t.infinite_tree.childTrees.get n
+      no_orphans := by intro ns; rw [InfiniteTreeSkeleton.get_get_childTrees]; intro eq_none n'; rw [InfiniteTreeSkeleton.get_childTrees, InfiniteTreeSkeleton.drop_drop]; apply t.no_orphans; exact eq_none
+      no_holes_in_children := by intro ns; rw [InfiniteTreeSkeleton.get_childTrees, InfiniteTreeSkeleton.drop_drop]; apply t.no_holes_in_children
+    }
+    no_holes := by intro n'; simp only [InfiniteList.get]; rw [PossiblyInfiniteTreeWithRoot.tree_to_opt_none_iff, PossiblyInfiniteTreeWithRoot.tree_to_opt_none_iff]; exact t.no_holes_in_children [] n'
+
+  theorem childTrees_empty {α} : (@PossiblyInfiniteTree.empty α).childTrees = PossiblyInfiniteList.empty := by rfl
+
+  def node (root : α) (childTrees : PossiblyInfiniteList (PossiblyInfiniteTreeWithRoot α)) : PossiblyInfiniteTree α where
+    infinite_tree := InfiniteTreeSkeleton.node (.some root) (childTrees.infinite_list.map (PossiblyInfiniteTree.infinite_tree ∘ PossiblyInfiniteTreeWithRoot.opt_to_tree))
     no_orphans := by
-      intro node
-      cases eq : node.all (fun e => e = 0) with
-      | false => simp
-      | true =>
-        intro not_none
-        intro parent
-        rcases parent.property with ⟨diff, node_eq⟩
-        have : parent.val.all (fun e => e = 0) := by
-          rw [← node_eq] at eq
-          rw [List.all_append] at eq
-          rw [Bool.and_eq_true] at eq
-          exact eq.right
-        simp only [this, ↓reduceIte]
-        cases diff with
-        | nil => rw [List.nil_append] at node_eq; rw [node_eq]; apply not_none
-        | cons _ _ =>
-          let parent_len_fin : Fin node.length := ⟨parent.val.length, by simp only [← node_eq, List.cons_append, List.length_cons, List.length_append]; apply Nat.lt_add_one_of_le; simp⟩
-          have := branch.no_holes node.length not_none parent_len_fin
-          exact this
+      intro ns
+      cases ns with
+      | nil => intro contra; rw [← InfiniteTreeSkeleton.root.eq_def, InfiniteTreeSkeleton.root_node] at contra; simp at contra
+      | cons n ns =>
+        rw [← InfiniteTreeSkeleton.childTrees.eq_def, InfiniteTreeSkeleton.childTrees_node]
+        intro eq_none n'
+        unfold InfiniteList.map at eq_none
+        rw [InfiniteTreeSkeleton.drop_node_cons, InfiniteList.get_map]
+        apply (PossiblyInfiniteTreeWithRoot.opt_to_tree (childTrees.infinite_list.get n)).no_orphans
+        exact eq_none
     no_holes_in_children := by
-      intro l n
-      unfold InfiniteTreeSkeleton.children
-      cases n with
-      | succ n =>
-        have all_eq_false : ((n+1)::l).all (fun e => e = 0) = false := by
-          rw [List.all_eq_false]
-          exists n+1
+      intro ns
+      cases ns with
+      | nil => rw [InfiniteTreeSkeleton.drop_nil]; unfold InfiniteTreeSkeleton.childNodes; rw [InfiniteTreeSkeleton.childTrees_node]; intro n; simp only [InfiniteList.get_map, Function.comp_apply]; rw [← PossiblyInfiniteTree.root.eq_def, ← PossiblyInfiniteTree.root.eq_def, ← PossiblyInfiniteTreeWithRoot.opt_to_tree_none_iff, ← PossiblyInfiniteTreeWithRoot.opt_to_tree_none_iff]; exact childTrees.no_holes n
+      | cons n ns =>
+        rw [InfiniteTreeSkeleton.drop_node_cons, InfiniteList.get_map]
+        exact (PossiblyInfiniteTreeWithRoot.opt_to_tree (childTrees.infinite_list.get n)).no_holes_in_children ns
+
+  theorem get?_node_nil {root : α} {childTrees : PossiblyInfiniteList (PossiblyInfiniteTreeWithRoot α)} : (node root childTrees).get? [] = .some root := by rfl
+  theorem get?_node_cons {root : α} {childTrees : PossiblyInfiniteList (PossiblyInfiniteTreeWithRoot α)} : ∀ n ns, (node root childTrees).get? (n :: ns) = (PossiblyInfiniteTreeWithRoot.opt_to_tree (childTrees.get? n)).get? ns := by intro n ns; rfl
+
+  theorem root_node {root : α} {childTrees : PossiblyInfiniteList (PossiblyInfiniteTreeWithRoot α)} : (node root childTrees).root = root := by rfl
+  theorem childTrees_node {root : α} {childTrees : PossiblyInfiniteList (PossiblyInfiniteTreeWithRoot α)} : (node root childTrees).childTrees = childTrees := by
+    unfold node PossiblyInfiniteTree.childTrees
+    simp only [InfiniteTreeSkeleton.childTrees_node, InfiniteList.get_map, Function.comp_apply]
+    apply PossiblyInfiniteList.ext
+    intro n
+    simp only [PossiblyInfiniteList.get?, InfiniteList.get]
+    rw [PossiblyInfiniteTreeWithRoot.tree_to_opt_after_opt_to_tree]
+
+  theorem node_root_childTrees {t : PossiblyInfiniteTree α} {root : α} (h : t.root = .some root) : t = node root t.childTrees := by
+    rw [PossiblyInfiniteTree.mk.injEq]; simp only [node]; rw [← h]; rw [InfiniteTreeSkeleton.node_root_childTrees t.infinite_tree]
+    apply congrArg
+    unfold PossiblyInfiniteTree.childTrees
+    apply InfiniteList.ext
+    intro n
+    simp only [InfiniteList.get_map, Function.comp_apply]
+    simp only [InfiniteList.get]
+    rw [PossiblyInfiniteTreeWithRoot.opt_to_tree_after_tree_to_opt]
+
+  theorem get?_childTrees {t : PossiblyInfiniteTree α} : ∀ n, (t.childTrees.get? n) = PossiblyInfiniteTreeWithRoot.tree_to_opt (t.drop [n]) := by intros; rfl
+  theorem get?_get?_childTrees {t : PossiblyInfiniteTree α} : ∀ n ns, (PossiblyInfiniteTreeWithRoot.opt_to_tree (t.childTrees.get? n)).get? ns = t.get? (n::ns) := by intros; rw [get?_childTrees, PossiblyInfiniteTreeWithRoot.opt_to_tree_after_tree_to_opt]; rfl
+
+  theorem drop_node_cons {root : α} {childTrees : PossiblyInfiniteList (PossiblyInfiniteTreeWithRoot α)} {n : Nat} {ns : List Nat} : (node root childTrees).drop (n::ns) = (PossiblyInfiniteTreeWithRoot.opt_to_tree (childTrees.get? n)).drop ns := by rfl
+
+  def childNodes (t : PossiblyInfiniteTree α) : PossiblyInfiniteList α where
+    infinite_list := t.infinite_tree.childNodes
+    no_holes := t.no_holes_in_children []
+
+  theorem get?_childNodes {t : PossiblyInfiniteTree α} : ∀ {n}, t.childNodes.get? n = (PossiblyInfiniteTreeWithRoot.opt_to_tree (t.childTrees.get? n)).root := by
+    intro n; rw [get?_childTrees, PossiblyInfiniteTreeWithRoot.opt_to_tree_after_tree_to_opt]; rfl
+
+  theorem childNodes_eq {t : PossiblyInfiniteTree α} : t.childNodes = t.childTrees.map (fun t => t.val.root.get (by rw [Option.isSome_iff_ne_none]; exact t.property)) := by
+    apply PossiblyInfiniteList.ext
+    intro n
+    rw [PossiblyInfiniteList.get?_map]
+    rw [get?_childNodes, get?_childTrees, PossiblyInfiniteTreeWithRoot.opt_to_tree_after_tree_to_opt]
+    apply Eq.symm
+    cases eq : (t.drop [n]).root with
+    | none => rw [Option.map_eq_none_iff, PossiblyInfiniteTreeWithRoot.tree_to_opt_none_iff]; exact eq
+    | some r => rw [Option.map_eq_some_iff]; exists ⟨t.drop [n], by simp [eq]⟩; rw [PossiblyInfiniteTreeWithRoot.tree_to_opt_some_iff]; simp [eq]
+
+  theorem childNodes_empty {α} : (@PossiblyInfiniteTree.empty α).childNodes = PossiblyInfiniteList.empty := by
+    apply PossiblyInfiniteList.ext; intro _; rw [get?_childNodes, childTrees_empty, PossiblyInfiniteList.get?_empty, PossiblyInfiniteList.get?_empty, ← PossiblyInfiniteTreeWithRoot.opt_to_tree_none_iff]
+
+  theorem no_orphans' {t : PossiblyInfiniteTree α} : ∀ ns : List Nat, t.get? ns = none -> ∀ n, (t.drop ns).childNodes.get? n = none := by exact t.no_orphans
+
+  theorem no_orphans'_closure {t : PossiblyInfiniteTree α} :
+      ∀ ns : List Nat, t.get? ns = none -> ∀ ns', (t.drop ns).get? ns' = none := by
+    exact t.infinite_tree.no_orphans_closure t.no_orphans
+
+  def branchForAddress (t : PossiblyInfiniteTree α) (ns : InfiniteList Nat) : PossiblyInfiniteList α where
+    infinite_list := t.infinite_tree.branchForAddress ns
+    no_holes := by
+      intro n
+      rw [InfiniteTreeSkeleton.get_branchForAddress]
+      intro eq_none
+      rw [InfiniteTreeSkeleton.get_branchForAddress]
+      rw [InfiniteList.take_succ']
+      apply t.no_orphans
+      exact eq_none
+
+  theorem get?_branchForAddress {t : PossiblyInfiniteTree α} {ns : InfiniteList Nat} {n : Nat} : (t.branchForAddress ns).get? n = t.get? (ns.take n) := by rfl
+
+  def branchAddressIsMaximal (t : PossiblyInfiniteTree α) (ns : InfiniteList Nat) : Prop :=
+    ∀ n, (t.branchForAddress ns).get? n.succ = none -> (t.drop (ns.take n)).childNodes.head = none
+
+  def branches (t : PossiblyInfiniteTree α) : Set (PossiblyInfiniteList α) :=
+    fun b => ∃ ns, b = t.branchForAddress ns ∧ t.branchAddressIsMaximal ns
+
+  theorem branches_eq {t : PossiblyInfiniteTree α} : t.branches = fun b =>
+      b.head = t.root ∧ ((t.childTrees = PossiblyInfiniteList.empty ∧ b.tail = PossiblyInfiniteList.empty) ∨ (∃ c ∈ t.childTrees, b.tail ∈ c.val.branches)) := by
+    unfold branches
+    apply Set.ext
+    intro b
+    constructor
+    . rintro ⟨ns, b_eq, ns_max⟩
+      constructor
+      . rw [b_eq]; rfl
+      . cases eq : t.childTrees.get? (ns.get 0) with
+        | none =>
+          apply Or.inl
+          rw [get?_childTrees] at eq
+          rw [PossiblyInfiniteTreeWithRoot.tree_to_opt_none_iff] at eq
+          rw [root_drop] at eq
+          rw [PossiblyInfiniteList.empty_iff_head_none]
+          rw [PossiblyInfiniteList.empty_iff_head_none]
           constructor
-          . apply List.mem_cons_self
-          . simp
-        simp [all_eq_false]
-      | zero =>
-        intro _ m
-        have isLt := m.isLt
-        simp at isLt
-  }
+          . specialize ns_max 0
+            rw [get?_branchForAddress] at ns_max
+            rw [InfiniteList.take_succ, InfiniteList.take_zero, InfiniteList.take_zero, drop_nil] at ns_max
+            unfold InfiniteList.head at ns_max
+            specialize ns_max eq
+            rw [PossiblyInfiniteList.head_eq] at ns_max
+            rw [PossiblyInfiniteList.head_eq]
+            rw [get?_childNodes, ← PossiblyInfiniteTreeWithRoot.opt_to_tree_none_iff] at ns_max
+            exact ns_max
+          . rw [b_eq]
+            rw [PossiblyInfiniteList.head_eq, PossiblyInfiniteList.get?_tail]
+            rw [get?_branchForAddress]
+            rw [InfiniteList.take_succ, InfiniteList.take_zero]
+            unfold InfiniteList.head
+            exact eq
+        | some c =>
+          apply Or.inr
+          exists c
+          constructor
+          . exists ns.get 0
+          exists ns.tail
+          rw [get?_childTrees] at eq
+          rw [PossiblyInfiniteTreeWithRoot.tree_to_opt_some_iff] at eq
+          constructor
+          . rw [b_eq]
+            apply PossiblyInfiniteList.ext
+            intro n
+            rw [PossiblyInfiniteList.get?_tail]
+            rw [get?_branchForAddress]
+            rw [get?_branchForAddress]
+            rw [InfiniteList.take_succ]
+            rw [← List.singleton_append]
+            rw [← get?_drop]
+            unfold InfiniteList.head
+            rw [eq.left]
+          . intro n
+            specialize ns_max (n+1)
+            rw [get?_branchForAddress] at ns_max
+            rw [InfiniteList.take_succ] at ns_max
+            rw [← List.singleton_append] at ns_max
+            rw [← get?_drop] at ns_max
+            unfold InfiniteList.head at ns_max
+            rw [eq.left] at ns_max
+            rw [get?_branchForAddress]
+            intro h
+            specialize ns_max h
+            rw [InfiniteList.take_succ] at ns_max
+            rw [← List.singleton_append] at ns_max
+            rw [← drop_drop] at ns_max
+            unfold InfiniteList.head at ns_max
+            rw [eq.left] at ns_max
+            exact ns_max
+    . rintro ⟨head_eq, tail_eq⟩
+      cases tail_eq with
+      | inl tail_eq =>
+        exists fun _ => 0
+        constructor
+        . apply PossiblyInfiniteList.ext
+          intro n
+          cases n with
+          | zero =>
+            rw [get?_branchForAddress, InfiniteList.take_zero]
+            exact head_eq
+          | succ n =>
+            rw [← PossiblyInfiniteList.get?_tail]
+            rw [tail_eq.right, PossiblyInfiniteList.get?_empty]
+            rw [get?_branchForAddress, InfiniteList.take_succ, ← List.singleton_append, ← get?_drop]
+            simp only [InfiniteList.head, InfiniteList.get]
+            have : t.childTrees.get? 0 = none := by rw [tail_eq.left, PossiblyInfiniteList.get?_empty]
+            rw [get?_childTrees, PossiblyInfiniteTreeWithRoot.tree_to_opt_none_iff] at this
+            rw [← empty_iff_root_none] at this
+            rw [this, get?_empty]
+        . intro n
+          rw [get?_branchForAddress, InfiniteList.take_succ', ← List.singleton_append, ← get?_drop]
+          simp only [InfiniteList.get, List.append_nil]
+          rw [PossiblyInfiniteList.head_eq]
+          rw [get?_childNodes]
+          rw [← PossiblyInfiniteTreeWithRoot.opt_to_tree_none_iff]
+          rw [get?_childTrees]
+          rw [PossiblyInfiniteTreeWithRoot.tree_to_opt_none_iff]
+          rw [root_drop]
+          intro h; exact h
+      | inr tail_eq =>
+        rcases tail_eq with ⟨c, c_mem, ns, tail_eq, ns_max⟩
+        rw [PossiblyInfiniteList.mem_iff] at c_mem
+        rcases c_mem with ⟨i, c_mem⟩
+        exists InfiniteList.cons i ns
+        rw [get?_childTrees] at c_mem
+        rw [PossiblyInfiniteTreeWithRoot.tree_to_opt_some_iff] at c_mem
+        constructor
+        . apply PossiblyInfiniteList.ext
+          intro n
+          rw [get?_branchForAddress]
+          cases n with
+          | zero => rw [InfiniteList.take_zero]; exact head_eq
+          | succ n =>
+            rw [← PossiblyInfiniteList.get?_tail, tail_eq]
+            rw [InfiniteList.take_succ, InfiniteList.head_cons, InfiniteList.tail_cons]
+            rw [← List.singleton_append]
+            rw [← get?_drop]
+            rw [c_mem.left]
+            rw [get?_branchForAddress]
+        . intro n
+          rw [get?_branchForAddress]
+          cases n with
+          | zero =>
+            intro contra
+            rw [InfiniteList.take_succ, InfiniteList.take_zero, InfiniteList.head_cons] at contra
+            rw [root_drop] at c_mem
+            rw [contra] at c_mem
+            simp at c_mem
+          | succ n =>
+            specialize ns_max n
+            rw [InfiniteList.take_succ, InfiniteList.head_cons, InfiniteList.tail_cons]
+            rw [← List.singleton_append]
+            rw [← get?_drop]
+            rw [c_mem.left]
+            rw [get?_branchForAddress] at ns_max
+            intro h; specialize ns_max h
+            rw [InfiniteList.take_succ, InfiniteList.head_cons, InfiniteList.tail_cons]
+            rw [← List.singleton_append]
+            rw [← drop_drop]
+            rw [c_mem.left]
+            exact ns_max
+
+  def leaves (t : PossiblyInfiniteTree α) : Set α := fun a => ∃ node : List Nat, t.get? node = some a ∧ (t.drop node).childNodes.head = none
+
+  def from_branch (b : PossiblyInfiniteList α) : PossiblyInfiniteTree α where
+    infinite_tree := fun ns => if ns.all (fun e => e = 0) then b.infinite_list ns.length else none
+    no_orphans := by
+      intro ns eq_none n
+      simp only [InfiniteTreeSkeleton.get] at eq_none
+      rw [InfiniteTreeSkeleton.get_childNodes, InfiniteTreeSkeleton.get_drop]
+      simp only [InfiniteTreeSkeleton.get]
+      cases eq : (ns ++ [n]).all (fun e => e = 0) with
+      | false => rfl
+      | true =>
+        have : ns.all (fun e => e = 0) := by rw [List.all_append, Bool.and_eq_true] at eq; exact eq.left
+        simp only [this] at eq_none
+        simp only [List.length_append, List.length_singleton]
+        apply b.no_holes
+        exact eq_none
+    no_holes_in_children := by
+      intro ns n _
+      rw [InfiniteTreeSkeleton.get_childNodes, InfiniteTreeSkeleton.get_drop]
+      simp only [InfiniteTreeSkeleton.get]
+      have : (ns ++ [n.succ]).all (fun e => e = 0) = false := by
+        rw [List.all_eq_false]
+        exists n.succ
+        simp
+      simp [this]
 
 end PossiblyInfiniteTree
 
